Add files via upload

summer_camp/List.lean
@@ -1,5 +1,11 @@
 /-
-  List type, join, filter, flatten
+  This Lean program defines List type, and
+  illustrate functional programming
+
+  We will see join, filter, and flatten in this program.
+
+  All examples can be repeated in Python. But in Python we cannot
+  do mathematical proof.
 -/
 
 
@@ -9,12 +15,61 @@ namespace hidden
 inductive List (A :Type)
   | nil
   | cons (a:A) (l: List A)
+  deriving Repr
+
+
+-- examples of list
+def list1 : List Nat := .cons 1 (.cons 2 (.cons 3 .nil))
+-- List.cons 1 (hidden.List.cons 2 (hidden.List.cons 3 (hidden.List.nil)))
+
+def list2 : List Nat := .cons 4 (.cons 5 .nil)
+-- List.cons 4 (hidden.List.cons 5 (hidden.List.nil))
+
+#eval list1
+#eval list2
+
+
+
+-- macro rules for defining and printing a term of type List
+macro_rules
+  -- Rule 1: Empty brackets translate to `nil`
+  | `([ ]) => `(List.nil)
+  -- Rule 2: A single item translates to `cons x nil`
+  | `([ $x ]) => `(List.cons $x List.nil)
+  -- Rule 3: Multiple items: pop the first item off, and recursively call the macro on the rest!
+  | `([ $x, $xs,*, $y ]) => `(List.cons $x [ $xs,*, $y ])
+  | `([ $x, $xs,* ]) => `(List.cons $x [ $xs,* ])
+
+-- Helper function: turns [| 1, 2 |] into the string "1, 2"
+def List.reprHelper {A : Type} [Repr A] : List A → Std.Format
+  | nil => ""
+  | cons a nil => repr a
+  | cons a as => repr a ++ ", " ++ reprHelper as
+
+-- Now we register it to Lean's `Repr` typeclass
+instance {A : Type} [Repr A] : Repr (List A) where
+  reprPrec l _ := "[" ++ List.reprHelper l ++ "]"
+
+def myEasyList : List Nat := [ 1, 2, 3 ]
+
+#eval myEasyList -- [1,2,3]
+#eval list1   -- [1,2,3]
+#eval list2   -- [4,5]
+
 
 -- 2. List Multiplication
 def List.mul {A : Type} : List A → List A → List A :=
  fun a b ↦ match a, b with
  | nil, b => b
  | cons a as, b => cons a (List.mul as b)
+
+-- Example of `mul`
+example : list1.mul list2 = .cons 1 (.cons 2 (.cons 3 (.cons 4 (.cons 5 .nil)))) := by
+  rfl
+
+#eval list1.mul list2 -- [1,2,3,4,5]
+
+
 
 -- List multiplication is associative
 theorem List.mul_assoc {A : Type} (a b c : List A) :
@@ -30,6 +85,18 @@ def List.map {A B : Type} (f : A → B)
   fun a ↦ match a with
   | nil => nil
   | cons x xs => cons (f x) (List.map f xs)
+
+-- Let's double every number in list1
+def double (n : Nat) : Nat := n * 2
+
+#eval List.map double list1 -- [2,4,6]
+
+example : List.map double list1 = .cons 2 (.cons 4 (.cons 6 .nil)) := by
+  rfl
+
+-- a prettier way to write the above example
+example : List.map double list1 = [2,4,6] := by
+  rfl
 
 
 -- 4. Monadic Join: Flattens a List of Lists using `mul`
@@ -53,10 +120,41 @@ def List.filter {A : Type} (p : A → Prop) [DecidablePred p]
   (l : List A) : List A :=
   List.join (List.map (guard p) l)
 
+-- Let's filter out only the even numbers from [1, 2, 3, 4, 5]
+def isEven (n : Nat) : Prop := n % 2 = 0
+
+-- make `n%2=0` decidable
+instance (n : Nat) : Decidable (isEven n) :=
+  -- Lean's core provides `inferInstance` to fetch the decidability of `x = y`.
+  -- We cast it to apply to our `isEven` definition.
+  inferInstanceAs (Decidable (n % 2 = 0))
+
+def list3 : List Nat := list1.mul list2  -- [1, 2, 3, 4, 5]
+
+#eval List.filter isEven list3
+
+example : List.filter isEven list3 = .cons 2 (.cons 4 .nil) := by
+  -- `rfl` will compute the join(map(guard)) logic
+  rfl
+
+-- the same example written more concisely
+example : List.filter isEven list3 = [2,4] := by rfl
+
+
 /-    Flattening is simply collapsing a List of Lists into a single List
     by multiplying (appending) them all together. -/
 def List.flatten {A : Type} (l : List (List A)) : List A :=
   List.join l
+
+def nested_list : List (List Nat) := .cons list1 (.cons list2 .nil)
+
+#eval nested_list   -- [[1, 2, 3], [4, 5]]
+#eval List.flatten nested_list
+
+-- The flattened nested_list is the same as [1,2,3,4,5]
+example : List.flatten nested_list = [1,2,3,4,5] := by rfl
+
+
 
 /-- flatMap is the cornerstone of functional programming.
     It maps a function that creates lists, and then flattens the result.
@@ -64,6 +162,18 @@ def List.flatten {A : Type} (l : List (List A)) : List A :=
 def List.flatMap {A B : Type} (f : A → List B) (l : List A) : List B :=
   List.flatten (List.map f l)
 
+
+def makePair (n : Nat) : List Nat := .cons n (.cons (n + 10) .nil)
+def shortList : List Nat := .cons 1 (.cons 2 .nil)
+
+#eval makePair 3  -- [3, 13]
+#eval shortList  --  [1, 2]
+#eval List.flatMap makePair shortList  -- [1, 11, 2, 12]
+
+-- prove that List.flatMap makePair shortList
+-- is equal to [1,11,2,12]
+example : List.flatMap makePair shortList = [1,11,2,12] := by
+  rfl
 
 -- 8. a theorem about flattening
 theorem join_mul {A : Type} (x y : List (List A)) :
@@ -88,5 +198,24 @@ theorem join_mul {A : Type} (x y : List (List A)) :
 theorem flatten_mul {A : Type} (x y : List (List A)) :
   List.flatten (x.mul y) = (List.flatten x).mul (List.flatten y) := by
   exact join_mul x y
+
+
+-- The theorem says:
+-- flatten([[1, 2]] * [[3], [4]]) = flatten([[1, 2]]) * flatten([[3], [4]])
+def nested1 : List (List Nat) := .cons (.cons 1 (.cons 2 .nil)) .nil
+def nested2 : List (List Nat) := .cons (.cons 3 .nil) (.cons (.cons 4 .nil) .nil)
+
+#eval nested1   -- [[1, 2]]
+#eval nested2   --[[3], [4]]
+#eval List.flatten (nested1.mul nested2)  -- [1,2,3,4]
+#eval (List.flatten nested1).mul (List.flatten nested2)  -- [1,2,3,4]
+
+
+example : List.flatten (nested1.mul nested2) = (List.flatten nested1).mul (List.flatten nested2) := by
+  -- We don't even need to compute it with `rfl`!
+  -- We can just apply the theorem `join_mul`
+  exact join_mul nested1 nested2
+
+
 
 end hidden
